FactoryGameStuff.v
@@ -1,0 +1,110 @@
+
+Set Implicit Arguments.
+Set Asymmetric Patterns.
+
+Require Import Unicode.Utf8.
+Require Import List.
+Require Import Vector.
+Import EqNotations.
+Require Import Coq.Program.Equality.
+Load EliUtils.
+(* Require Import Eli.EliUtils.
+
+Locate "<". *)
+
+Notation "a ∈ c" := (In a c) (at level 60, no associativity) : type_scope.
+Notation "a ∉ c" := (¬In a c) (at level 60, no associativity) : type_scope.
+
+Definition Graph n := Vector.t (list (Fin.t n)) n.
+
+Definition HasPredecessorLeft n (graph : Graph n) (partial_result : list (Fin.t n)) (node : Fin.t n) :=
+  ∃ (predecessor : Fin.t n) (edge : listIndex (Vector.nth graph predecessor)), predecessor ∉ partial_result ∧ valueAt edge = node.
+  
+Inductive TopoStep n (graph : Graph n) (partial_result : list (Fin.t n)) :=
+| TopoStepDone (_: ∀ node, HasPredecessorLeft graph partial_result node)
+| TopoStepPush next (_: ¬HasPredecessorLeft graph partial_result next).
+
+Inductive PartialTopoSort n (graph : Graph n) : list (Fin.t n) → Prop :=
+| TopoSortNil : PartialTopoSort graph nil
+| TopoSortCons partial_result next (_: ¬HasPredecessorLeft graph partial_result next) : PartialTopoSort graph (next :: partial_result).
+
+Definition TopoSort n (graph : Graph n) (partial_result : list (Fin.t n)) : Prop := PartialTopoSort graph partial_result ∧ ∀ node, HasPredecessorLeft graph partial_result node.
+
+Lemma PartialTopoSort_is_topological
+  n (graph : Graph n) partial_result (sort : PartialTopoSort graph partial_result)
+  : 
+  (* "If there's an edge from i0 to i1, i1 must come first" *)
+  ∀ (i0 i1 : listIndex partial_result) (edge : listIndex (Vector.nth graph (valueAt i0))),
+    valueAt edge = valueAt i1 →
+    positionOf i1 < positionOf i0.
+  admit.
+Admitted.  
+
+
+(*
+  
+Definition graphRemove n
+  (graph: Graph n)
+  (removed : Fin.t n)
+  : list (list nat)
+  := replaceAt removed nil.
+  
+  
+Lemma graphRemoveValid
+  (output_edges : list (list nat))
+  (output_edges_valid : ∀ (i : listIndex output_edges) (j : listIndex (valueAt i)), valueAt j < length output_edges)
+  (removed : listIndex output_edges)
+  : let result_edges := (graphRemove removed) in
+    ∀ (i : listIndex result_edges) (j : listIndex (valueAt i)), valueAt j < length result_edges.
+  intros.
+  induction removed; cbn in *.
+  
+  dependent destruction i; cbn in *.
+  easy.
+  exact (output_edges_valid (there head i) j).
+  
+  unfold graphRemove in IHremoved; rewrite (replaceRetainsLength removed nil) in *; dependent destruction i; cbn in *.
+  exact (output_edges_valid (here head tail) j).
+  admit.
+Admitted.
+
+Inductive TopoSort 
+  (output_edges : list (list nat))
+  (output_edges_valid : ∀ (i : listIndex output_edges) (j : listIndex (valueAt i)), valueAt j < length output_edges) :=
+| Done (_: ∀ (node : listIndex output_edges), ∃ (predecessor : listIndex output_edges) (edge : listIndex (valueAt predecessor)), predecessor ≠ node ∧ valueAt edge = positionOf node)
+| Step (first : listIndex output_edges) (rest : TopoSort (graphRemoveValid output_edges_valid first)).
+
+
+Record TopoSortStep := mkTopoSortStep
+  { output_edges : Memory
+  ; output_edges_valid : list (ThreadId × list Instruction)
+  }.
+  
+  
+Record topo_step :
+  (output_edges : list (list nat))
+  (output_edges_valid : ∀ i j k l , output_edges[i] = l → l[j] = k → k < length output_edges)
+  
+  
+  
+
+Definition topological_ordering_of_noncyclic_machines
+  (output_edges : list (list nat))
+  (output_edges_valid : ∀ i j k l , output_edges[i] = l → l[j] = k → k < length output_edges)
+  : list nat.
+  admit.
+Admitted.
+
+Lemma topological_ordering_is_topological
+  (output_edges : list (list nat))
+  (output_edges_valid : ∀ i j k l , output_edges[i] = l → l[j] = k → k < length output_edges)
+  : let result := topological_ordering_of_noncyclic_machines output_edges_valid in
+  ∀ o0 o1 m0 m1 l i,
+    result[o0] = m0 →
+    result[o1] = m1 →
+    output_edges[m0] = l →
+    l[i] = m1 →
+    o0 < o1.
+  admit.
+Admitted.
+  *)
